Implementation, Specification and Lemma finished for 2to1 n-bit multiplexer. Appended to TODO.

src/Combinational.lean
@@ -1,5 +1,6 @@
-import Gates tactic Conversions data.vector data.real.basic
+import Gates tactic Conversions data.vector data.real.basic Sequential
 
+--2to1 mux with 1 bit input
 def mux_imp (in1 in2 sel out : bool) : Prop :=
 	∃ (p q r : bool), (nand_n [in1, p] q) ∧ (nand_n [sel, in2] r) ∧ 
 		(nand_n [q, r] out) ∧ (not_ sel p)
@@ -7,6 +8,14 @@ def mux_imp (in1 in2 sel out : bool) : Prop :=
 def mux_spec (in1 in2 sel out : bool) : Prop :=
 	if sel then (out = in2) else (out = in1) 
 
+--2to1 mux with n-bit inputs
+def mux_n_spec {n : ℕ} (in1 in2 : array n bool) (sel : bool) (out : array n bool) : Prop :=
+	∀ i : fin n, if sel then (out.read i = in2.read i) else (out.read i = in1.read i) 
+
+def mux_n_imp {n : ℕ} (in1 in2 : array n bool) (sel : bool) (out : array n bool) : Prop :=
+	∀ i : fin n, mux_imp (in1.read i) (in2.read i) sel (out.read i)
+
+--2to4 decoder
 def dec_imp (in0 in1 out0 out1 out2 out3 : bool) : Prop :=
 	∃ (p q : bool), (not_ in0 p) ∧ (not_ in1 q) ∧ (and_n [p, q] out0) ∧ 
 		(and_n [in0, q] out1) ∧ (and_n [p, in1] out2) ∧ (and_n [in0, in1] out3)
@@ -16,4 +25,5 @@ def dec_spec (in0 in1 out0 out1 out2 out3 : bool) : Prop :=
 	else if ¬in1 ∧ in0 then (out3 = ff ∧ out2 = ff ∧ out1 = tt ∧ out0 = ff)
 	else if in1 ∧ ¬in0 then (out3 = ff ∧ out2 = tt ∧ out1 = ff ∧ out0 = ff)
 	else (out3 = tt ∧ out2 = ff ∧ out1 = ff ∧ out0 = ff)
+
 
