README.md
@@ -2,14 +2,26 @@
 Verification of combinational and sequential circuits in LEAN3
 
 ### Column Name
-- [ ] ... 
-  - [ ] ...  
-
+- [ ] Full-adder 
+  - [ ] Implementation on single boolean  
+  - [ ] Specification on single boolean  
+  - [ ] Lemma on single booleans  
+  - [ ] Implementation on n-bit wide booleans  
+  - [ ] Specification on n-bit wide booleans
+  - [ ] Lemma on n-bit wide booleans
+- [ ] N-bit counter
+  - [ ] Implementation on n-bit wide booleans  
+  - [ ] Specification on n-bit wide booleans
+  - [ ] Lemma on n-bit wide booleans
+  
 ### Completed Column ✓
 - [x] Logic Gates on single booleans
 - [x] 2to1 Mux Implementation on single boolean
 - [x] 2to1 Mux Specification on single boolean
 - [x] 2to1 Mux Lemma on single booleans
+- [x] 2to1 Mux Implementation on n-bit wide booleans
+- [x] 2to1 Mux Specification on n-bit wide booleans
+- [x] 2to1 Mux Lemma on n-bit wide booleans
 - [x] Memory Implementation single boolean
 - [x] Memory Specification single boolean
 - [x] Memory Lemma single boolean
